\documentclass{article}
\usepackage[utf8]{inputenc}
\usepackage{polski}


\usepackage{amssymb, amsmath, amsfonts, amsthm, cite, mathtools, enumerate, rotating, hyperref}
\newcommand \eq[1]{\begin{equation} \begin{split}  #1 \end{split} \end{equation}}


\makeatletter
\def\@seccntformat#1{%
  \expandafter\ifx\csname c@#1\endcsname\c@section\else
  \csname the#1\endcsname\quad
  \fi}
\makeatother

\title{}
\date{31.03.2020}
\author{Maurycy Borkowski}
\begin{document}
\maketitle

\section{L5Z3 (3 punkty)}
Błąd został popełniony tu:
$$
\frac{d}{dx}\left(\frac{\cos{x}}{\sin^2{x}}\right) = \frac{-\sin x \sin^2 x - \cos x 2 \sin x \cos x}{\sin^4 x} = \frac{-\sin x (\sin^2 x + 2 \cos^2 x)}{\sin^4 x} =
$$
$$
= \frac{1 + \cos^2 x}{\sin^3 x} \neq \frac{1- \cos^2 x}{\sin^3 x} = \frac{\sin^2 x}{\sin^3 x} = \frac{1}{\sin x}
$$
\\\\\\
\section{L5Z4 (10 punktów)}
\begin{proof}
Skoro $f(x)$ i $g(x)$ rosnące to dla dowolnych $a,b \in [0,1]$:
$$
(f(a) - f(b))(g(a)-g(b)) \geq 0
$$
Dalej:
$$
\int_0^1 \int_0^1 (f(x) - f(y))(g(x)-g(y)) dxdy \geq 0
$$
$$
\int_0^1 \int_0^1 (f(x)g(x) + f(y)g(y) - [f(x)g(y) + f(y)g(x)]) dxdy \geq 0
$$
$$
(1-0)\left(\int_0^1 f(x)g(x)dx  + \int_0^1 f(y)g(y)dy \right)- \int_0^1 \int_0^1 [f(x)g(y) + f(y)g(x)) dxdy \geq 0
$$
$$
2\int_0^1 f(x)g(x)dx  - \int_0^1 g(y) \left(\int_0^1 f(x)dx\right)dy - \int_0^1 f(y) \left(\int_0^1 g(x)dx\right)dy\geq 0
$$
$$
2\int_0^1 f(x)g(x)dx  - 2\int_0^1 g(x)dx \int_0^1  f(x)dx\geq 0
$$
$$
\int_0^1 f(x)g(x)dx  \geq \int_0^1 g(x)dx \int_0^1  f(x)dx
$$
\end{proof}
\end{document}

% Nieużywane Kursory